get rid of some admits; other small cleanups

tmonad/size_linear.v
@@ -1,16 +1,11 @@
-Require Import Braun.tmonad.monad.
+Require Import Braun.tmonad.monad Braun.common.big_oh.
 Require Import Braun.common.braun Braun.common.util.
 Require Import Omega.
 
 Section size_linear.
   Variable A : Set.
 
-  Definition size_linear_rt n : nat :=
-    match n with 
-      | 0   => 3
-      (* Placeholder, Obviously wrong! *)
-      | S n => 0
-    end.
+  Definition size_linear_rt n : nat := 13 * n + 3.
 
   Definition size_linear_result (bt : @bin_tree A) (n:nat) c :=
     c = size_linear_rt n /\ (forall m, Braun bt m -> m = n).
@@ -27,33 +22,32 @@ Section size_linear.
 
   Next Obligation.
   Proof.
-    (* Why are there duplicated premises? 
-  A : Set
-  x : A
-  l : bin_tree
-  r : bin_tree
-  lsize : nat
-  xm : nat
-  H3 : size_linear_result l lsize xm
-  rsize : nat
-  xm0 : nat
-  H2 : size_linear_result r rsize xm0
-  xn : nat
-  H0 : size_linear_result r rsize xn
-  xn0 : nat
-  H1 : size_linear_result l lsize xn0
-  ============================
-   size_linear_result (bt_node x l r) (lsize + rsize + 1) (xn0 + (xn + 10))
-     *)
-    
+    clear xm0 H2 xm H3.
+    rename H0 into SLRr.
+    rename H1 into SLRl.
+
+    destruct SLRr as [XNeq Br].
+    destruct SLRl as [XN0eq Bl].
+    subst xn xn0.
+    unfold size_linear_result.
 
     split.
     (* Need to figure out what this supposed to be first *)
-    admit.
+    unfold size_linear_rt.
+    omega.
 
     intros m B. 
     invclr B.
-    destruct H2; destruct H3.
     auto.
   Qed.
+
+  Theorem size_linear_rt_is_linear : big_oh size_linear_rt (fun n => n).
+  Proof.
+    exists 1.
+    exists 16.
+    intros n LE.
+    unfold size_linear_rt.
+    omega.
+  Qed.
+
 End size_linear.
